WIP

src/ra/ObligationRA.v
@@ -256,16 +256,25 @@ Qed.
 
 Module ObligationRA.
 
-  Definition t: URA.t := @FiniteMap.t (@CounterRA.t Ord.t _).
+  Variant _unit : Type := _tt.
+
+  Definition t: URA.t := @FiniteMap.t (URA.prod (@CounterRA.t Ord.t _) (OneShot.t _unit)).
 
   Section RA.
     Context `{@GRA.inG t Σ}.
 
     Definition black (k: nat) (o: Ord.t): iProp :=
-      OwnM (FiniteMap.singleton k ((CounterRA.black o: @CounterRA.t Ord.t _): (@CounterRA.t Ord.t _))).
+      OwnM (FiniteMap.singleton k ((CounterRA.black o: @CounterRA.t Ord.t _, ε: OneShot.t _unit): URA.prod (@CounterRA.t Ord.t _) (OneShot.t _unit))).
 
     Definition white (k: nat) (o: Ord.t): iProp :=
-      OwnM (FiniteMap.singleton k ((CounterRA.white o: @CounterRA.t Ord.t _): (@CounterRA.t Ord.t _))).
+      OwnM (FiniteMap.singleton k ((CounterRA.white o: @CounterRA.t Ord.t _, ε: OneShot.t _unit): URA.prod (@CounterRA.t Ord.t _) (OneShot.t _unit))).
+
+    Definition pending (k: nat) (q: Qp): iProp :=
+      OwnM (FiniteMap.singleton k ((ε: @CounterRA.t Ord.t _, OneShot.pending _unit q: OneShot.t _unit): URA.prod (@CounterRA.t Ord.t _) (OneShot.t _unit))).
+
+    Definition shot (k: nat): iProp :=
+      OwnM (FiniteMap.singleton k ((ε: @CounterRA.t Ord.t _, OneShot.shot _tt: OneShot.t _unit): URA.prod (@CounterRA.t Ord.t _) (OneShot.t _unit))).
+
 
     Definition white_one k: iProp :=
       white k (Ord.S Ord.O).
@@ -286,19 +295,103 @@ Module ObligationRA.
       i. iIntros "POS". iPoseProof (black_persistent with "POS") as "POS". auto.
     Qed.
 
+    Lemma shot_persistent k
+      :
+      shot k -∗ □ shot k.
+    Proof.
+      iIntros "H".
+      unfold black.
+      iPoseProof (own_persistent with "H") as "H".
+      rewrite FiniteMap.singleton_core. auto.
+    Qed.
+
+    Global Program Instance Persistent_shot k: Persistent (shot k).
+    Next Obligation.
+    Proof.
+      i. iIntros "POS". ss. iPoseProof (shot_persistent with "POS") as "POS". auto.
+    Qed.
+
+    Lemma pending_shot k
+      :
+      (pending k 1)
+        -∗
+        #=> (shot k).
+    Proof.
+      iApply OwnM_Upd. eapply FiniteMap.singleton_updatable.
+      apply URA.prod_updatable.
+      { reflexivity. }
+      { apply OneShot.pending_shot. }
+    Qed.
+
+    Lemma pending_not_shot k q
+      :
+      (pending k q)
+        -∗
+        (shot k)
+        -∗
+        False.
+    Proof.
+      iIntros "H0 H1". iCombine "H0 H1" as "H".
+      iOwnWf "H". rewrite FiniteMap.singleton_add in H0.
+      rewrite FiniteMap.singleton_wf in H0.
+      ur in H0. des. exfalso. eapply OneShot.pending_not_shot; eauto.
+    Qed.
+
+    Lemma pending_sum k q0 q1
+      :
+      (pending k q0)
+        -∗
+        (pending k q1)
+        -∗
+        (pending k (q0 + q1)%Qp).
+    Proof.
+      iIntros "H0 H1". iCombine "H0 H1" as "H".
+      rewrite FiniteMap.singleton_add.
+      ur. rewrite URA.unit_id. ur. auto.
+    Qed.
+
+    Lemma pending_wf k q
+      :
+      (pending k q)
+        -∗
+        (⌜(q ≤ 1)%Qp⌝).
+    Proof.
+      iIntros "H". iOwnWf "H".
+      rewrite FiniteMap.singleton_wf in H0. ur in H0. des.
+      apply OneShot.pending_wf in H1. auto.
+    Qed.
+
+    Lemma pending_split k q0 q1
+      :
+      (pending k (q0 + q1)%Qp)
+        -∗
+        (pending k q0 ∗ pending k q1).
+    Proof.
+      iIntros "H".
+      iPoseProof (OwnM_extends with "H") as "[H0 H1]"; [|iSplitL "H0"; [iApply "H0"|iApply "H1"]].
+      { rewrite FiniteMap.singleton_add.
+        rewrite OneShot.pending_sum. ur.
+        rewrite URA.unit_id. ur. reflexivity.
+      }
+    Qed.
+
     Lemma alloc o
       :
-      ⊢ #=> (∃ k, black k o ∗ white k o).
+      ⊢ #=> (∃ k, black k o ∗ white k o ∗ pending k 1).
     Proof.
       iPoseProof (@OwnM_unit _ _ H) as "H".
       iPoseProof (OwnM_Upd_set with "H") as "> H0".
       { eapply FiniteMap.singleton_alloc.
-        instantiate (1:=((CounterRA.black o): (@CounterRA.t Ord.t _)) ⋅ ((CounterRA.white o): (@CounterRA.t Ord.t _))).
-        eapply CounterRA.black_white_wf.
+        instantiate (1:=((CounterRA.black o, ε): URA.prod (@CounterRA.t Ord.t _) (OneShot.t _unit)) ⋅ ((CounterRA.white o, ε): URA.prod (@CounterRA.t Ord.t _) (OneShot.t _unit)) ⋅ (ε, OneShot.pending _unit 1)).
+        repeat rewrite unfold_prod_add. repeat rewrite URA.unit_idl. repeat rewrite URA.unit_id.
+        rewrite unfold_prod_wf. ss. split.
+        { eapply CounterRA.black_white_wf. }
+        { apply OneShot.pending_one_wf. }
       }
       iDestruct "H0" as "[% [% H0]]".
-      des. subst. erewrite <- FiniteMap.singleton_add.
-      iDestruct "H0" as "[H0 H1]". iModIntro. iExists _. iFrame.
+      des. subst. erewrite <- FiniteMap.singleton_add. erewrite <- FiniteMap.singleton_add.
+      iDestruct "H0" as "[[H0 H1] H2]".
+      iModIntro. iExists _. iFrame.
     Qed.
 
     Lemma black_mon o1 k o0
@@ -307,6 +400,7 @@ Module ObligationRA.
       black k o0 -∗ black k o1.
     Proof.
       iApply OwnM_extends. apply FiniteMap.singleton_extends.
+      apply URA.prod_extends. split; [|reflexivity].
       apply CounterRA.black_mon. auto.
     Qed.
 
@@ -316,6 +410,7 @@ Module ObligationRA.
       white k o1 -∗ #=> white k o0.
     Proof.
       iApply OwnM_Upd. apply FiniteMap.singleton_updatable.
+      apply URA.prod_updatable; [|reflexivity].
       apply CounterRA.white_mon. auto.
     Qed.
 
@@ -338,7 +433,9 @@ Module ObligationRA.
       iIntros "H0 H1". unfold white.
       replace (CounterRA.white (Hessenberg.add o0 o1): @CounterRA.t Ord.t ord_OrderedCM) with
         ((CounterRA.white o0: @CounterRA.t Ord.t _) ⋅ (CounterRA.white o1: @CounterRA.t Ord.t _)).
-      { iCombine "H0 H1" as "H". rewrite FiniteMap.singleton_add. auto. }
+      { iCombine "H0 H1" as "H". rewrite FiniteMap.singleton_add.
+        rewrite unfold_prod_add. rewrite URA.unit_id. auto.
+      }
       { symmetry. eapply (@CounterRA.white_split Ord.t ord_OrderedCM o0 o1). }
     Qed.
 
@@ -349,10 +446,12 @@ Module ObligationRA.
         (white k o0 ∗ white k o1).
     Proof.
       iIntros "H". unfold white.
-      replace (CounterRA.white (Hessenberg.add o0 o1): @CounterRA.t Ord.t ord_OrderedCM) with
-        (((CounterRA.white o0): (@CounterRA.t Ord.t _)) ⋅ ((CounterRA.white o1): (@CounterRA.t Ord.t _))).
+      replace (CounterRA.white (Hessenberg.add o0 o1): @CounterRA.t Ord.t ord_OrderedCM, ε: @OneShot.t _unit) with
+        (((CounterRA.white o0, ε): URA.prod (@CounterRA.t Ord.t _) (OneShot.t _unit)) ⋅ ((CounterRA.white o1, ε): URA.prod (@CounterRA.t Ord.t _) (OneShot.t _unit))).
       { rewrite <- FiniteMap.singleton_add. iDestruct "H" as "[H0 H1]". iFrame. }
-      { symmetry. eapply (@CounterRA.white_split Ord.t ord_OrderedCM o0 o1). }
+      { rewrite unfold_prod_add. rewrite URA.unit_id. f_equal.
+        symmetry. eapply (@CounterRA.white_split Ord.t ord_OrderedCM o0 o1).
+      }
     Qed.
 
     Lemma white_split o0 o1 k o
@@ -403,6 +502,8 @@ Module ObligationRA.
       iCombine "H0 H1" as "H". rewrite FiniteMap.singleton_add.
       iOwnWf "H". iPureIntro.
       apply FiniteMap.singleton_wf in H0.
+      rewrite ! unfold_prod_add in H0.
+      rewrite unfold_prod_wf in H0. des. ss.
       apply CounterRA.black_white_compare in H0. auto.
     Qed.
 
@@ -417,8 +518,13 @@ Module ObligationRA.
       iIntros "H0 H1".
       iCombine "H0 H1" as "H". rewrite FiniteMap.singleton_add.
       iPoseProof (OwnM_Upd_set with "H") as "> [% [% H]]".
-      { eapply FiniteMap.singleton_updatable_set. eapply CounterRA.black_white_decr. }
-      { ss. des. subst. iModIntro. iExists _. iFrame. eauto. }
+      { eapply FiniteMap.singleton_updatable_set.
+        rewrite unfold_prod_add. eapply URA.prod_updatable_set.
+        { eapply CounterRA.black_white_decr. }
+        { instantiate (1:=eq (ε ⋅ ε: OneShot.t _unit)). ii. esplits; eauto. }
+      }
+      { ss. des. destruct m1. des; subst.
+        rewrite URA.unit_id. iModIntro. iExists _. iFrame. eauto. }
     Qed.
 
     Lemma black_white_decr_one k o1
@@ -451,6 +557,7 @@ Module ObligationRA.
       iPoseProof (black_white_decr_one with "H0 H2") as "> [% [H0 %]]".
       iModIntro. iExists _. iFrame. auto.
     Qed.
+
   End RA.
 
   Section EDGE.
@@ -546,7 +653,6 @@ Module ObligationRA.
 
   End EDGE.
 
-  Variant _unit : Type := _tt.
 
   Section ARROW.
     Variable (S: Type).
@@ -570,15 +676,58 @@ Module ObligationRA.
       fun '(i, k, c, q, x, f) =>
         ((□ (prop _ f -∗ □ (prop _ f)))
            ∗
-           ((OwnM (FiniteMap.singleton x (OneShot.shot _tt)) ∗ (prop _ f))
+           (((pending k (1/2)) ∗ (∃ n, FairRA.black Prism.id i n q) ∗ (white k (Jacobsthal.mult c Ord.omega)))
             ∨
-              (∃ n, (FairRA.black Prism.id i n q)
-                      ∗ white k (Jacobsthal.mult c (Ord.from_nat n)))))%I.
+              ((shot k)
+                 ∗
+                 ((OwnM (FiniteMap.singleton x (OneShot.shot _tt)) ∗ (prop _ f))
+                  ∨
+                    (∃ n, (FairRA.black Prism.id i n q)
+                            ∗ (white k (Jacobsthal.mult c (Ord.from_nat n)))))))
+        )%I.
 
     Definition arrows_sat: iProp := Regions.sat _ arrow.
 
-    Definition correl (i: Id) (k: nat) (c: Ord.t) (f : Var): iProp :=
+    Definition delay (i: Id) (k: nat) (c: Ord.t) (f : Var): iProp :=
       (∃ r q x, Regions.white _ r (Prism.review p i, k, c, q, x, f))%I.
+
+    Lemma delay_persistent i k c F
+      :
+      delay i k c F ⊢ □ delay i k c F.
+    Proof.
+      iIntros "# H". auto.
+    Qed.
+
+    Global Program Instance Persistent_delay i k c F: Persistent (delay i k c F).
+
+    Local Transparent IUpd.
+
+    Lemma delay_shot i k c F
+      :
+      (delay i k c F)
+        -∗
+        (pending k (1/2))
+        -∗
+        (#=(arrows_sat)=> (delay i k c F) ∗ (shot k)).
+    Proof.
+      iIntros "(% & % & % & #WHITE) P". 
+      iApply (Regions.update with "WHITE [P]").
+      iIntros "[#PERS [(PEND & BL & WH) | (#SHOT & _)]]".
+      { iMod (pending_shot with "[P PEND]") as "#SHOT".
+        { iEval (rewrite <- (Qp.div_2 1)). iApply (pending_sum with "P PEND"). }
+        iDestruct "BL" as "(% & BL)". iMod (white_mon _ _ (o0:=(c × (Ord.from_nat n))%ord) with "WH") as "WH".
+        Unshelve.
+        2:{ apply Jacobsthal.le_mult_r. apply Ord.lt_le. apply Ord.omega_upperbound. }
+        iModIntro. iSplitL.
+        { iEval (unfold arrow). iSplitR. auto. iRight. iSplitR. auto. iRight. iExists _. iFrame. }
+        { iSplitL. 2: auto. unfold delay. iExists _, _, _. eauto. }
+      }
+      { iPoseProof (pending_not_shot with "P SHOT") as "%FAL". inv FAL. }
+    Qed.
+
+
+    Definition correl (i: Id) (k: nat) (c: Ord.t) (f : Var): iProp :=
+      (shot k ∗ ∃ r q x, Regions.white _ r (Prism.review p i, k, c, q, x, f))%I.
 
     Lemma correl_persistent i k c F
       :
@@ -589,7 +738,26 @@ Module ObligationRA.
 
     Global Program Instance Persistent_correl i k c F: Persistent (correl i k c F).
 
-    Local Transparent IUpd.
+    Lemma delay_to_correl i k c F
+      :
+      (delay i k c F)
+        -∗
+        (shot k)
+        -∗
+        (correl i k c F).
+    Proof.
+      iIntros "D S". iFrame.
+    Qed.
+
+    Lemma unfold_correl i k c F
+      :
+      (correl i k c F)
+        -∗
+        (delay i k c F) ∗ (shot k).
+    Proof.
+      iIntros "[D S]". iFrame.
+    Qed.
+
     Lemma correl_correlate_gen i k c f n
       :
       (correl i k c f)
@@ -600,14 +768,15 @@ Module ObligationRA.
            ((□ (prop _ f -∗ □ (prop _ f)))
               ∗
               ((white k (Jacobsthal.mult c (Ord.from_nat n)))
-            ∨
-              (□ prop _ f)))).
+               ∨
+                 (□ prop _ f)))).
     Proof.
-      iIntros "[% [% [% WHITE]]] H".
+      iIntros "(#SHOT & [% [% [% WHITE]]]) H".
       iApply (Regions.update with "WHITE [H]").
-      iIntros "[#PERS [[OWN PROP]|[% [BLACK WHITE]]]]".
+      iIntros "[#PERS [[PEND _] | (_ & [[OWN PROP] | [% [BLACK WHITE]]])]]".
+      { iPoseProof (pending_not_shot with "PEND SHOT") as "%FAL". inv FAL. }
       { iModIntro. iPoseProof ("PERS" with "PROP") as "#F". iSplitL.
-        { iSplitR. auto. iLeft. iFrame. }
+        { iSplitR. auto. iRight. iSplitR. auto. iLeft. iFrame. }
         { iSplit. auto. iRight. auto. }
       }
       { iPoseProof (FairRA.decr_update with "BLACK H") as "> [% [H %]]".
@@ -617,7 +786,7 @@ Module ObligationRA.
           rewrite ClassicJacobsthal.mult_dist. reflexivity.
         }
         iModIntro. iSplitR "WHITE0".
-        { iSplitR. auto. iRight. iExists _. iFrame. }
+        { iSplitR. auto. iRight. iSplitR. auto. iRight. iExists _. iFrame. }
         { iSplit. auto. iLeft. auto. }
       }
     Qed.
@@ -787,12 +956,12 @@ Module ObligationRA.
       des; clarify. iApply IHrs; auto.
     Qed.
 
-    Lemma duty_correl i l k c f
+    Lemma duty_delay i l k c f
           (IN: List.In (k, c, f) l)
       :
       (duty i l)
         -∗
-        (correl i k c f).
+        (delay i k c f).
     Proof.
       iIntros "[% [% [BLACK [DUTY %]]]]".
       subst. eapply in_map_iff in IN. des. des_ifs.
@@ -800,19 +969,37 @@ Module ObligationRA.
       iExists _, _, _. iApply "WHITES". iPureIntro. eauto.
     Qed.
 
+    Lemma duty_correl i l k c f
+          (IN: List.In (k, c, f) l)
+      :
+      (duty i l)
+        -∗
+        (shot k)
+        -∗
+        (correl i k c f).
+    Proof.
+      iIntros "[% [% [BLACK [DUTY %]]]] #SHOT".
+      subst. eapply in_map_iff in IN. des. des_ifs.
+      iPoseProof (duty_list_whites with "DUTY") as "# WHITES".
+      iSplitR. auto. iExists _, _, _. iApply "WHITES". iPureIntro. eauto.
+    Qed.
+
     Lemma duty_done i l k c f
       :
       (duty i ((k, c, f)::l))
+        -∗
+        (shot k)
         -∗
         (prop _ f)
         -∗
         #=(arrows_sat)=> (duty i l).
     Proof.
-      iIntros "[% [% [BLACK [DUTY %]]]] PROP".
+      iIntros "[% [% [BLACK [DUTY %]]]] #SHOT PROP".
       destruct rs; ss. des_ifs.
       iPoseProof (duty_list_unfold with "DUTY") as "[WHITE [OWN DUTY]]".
       iPoseProof (Regions.update with "WHITE [OWN PROP]") as "> BLACKF".
-      { iIntros "[#PERS [[DONE _]|[% [BLACK WHITE]]]]".
+      { iIntros "[#PERS [(PEND & _) | (_ & [[DONE _]|[% [BLACK WHITE]]])]]".
+        { iPoseProof (pending_not_shot with "PEND SHOT") as "%FAL". inv FAL. }
         { iCombine "OWN DONE" as "FALSE".
           rewrite FiniteMap.singleton_add. iOwnWf "FALSE".
           rewrite FiniteMap.singleton_wf in H3.
@@ -821,10 +1008,8 @@ Module ObligationRA.
         iPoseProof (OwnM_Upd with "OWN") as "> OWN".
         { apply FiniteMap.singleton_updatable. apply OneShot.pending_shot. }
         iModIntro. iSplitR "BLACK".
-        { iSplitR. auto. iLeft. iFrame. }
-        { instantiate (1:=FairRA.black_ex p i q0).
-          iExists _. iApply "BLACK".
-        }
+        { iSplitR. auto. iRight. iSplit. auto. iLeft. iFrame. }
+        { instantiate (1:=FairRA.black_ex p i q0). iExists _. iApply "BLACK". }
       }
       iModIntro. iExists _, _. iSplitR "DUTY".
       { iApply (FairRA.black_ex_sum with "BLACK BLACKF"). }
@@ -837,24 +1022,22 @@ Module ObligationRA.
         -∗
         (white k (Jacobsthal.mult c Ord.omega))
         -∗
+        (pending k (1/2))
+        -∗
         (□ (prop _ f -∗ □ prop _ f))
         -∗
         #=(arrows_sat)=> (duty i ((k, c, f)::l)).
     Proof.
-      iIntros "[% [% [BLACK [DUTY %]]]] SHOT #PERS".
+      iIntros "[% [% [BLACK [DUTY %]]]] SHOT PEND #PERS".
       iPoseProof (FairRA.black_ex_split with "[BLACK]") as "[BLACK0 [% BLACK1]]".
       { rewrite Qp.div_2. iFrame. }
       iPoseProof (@OwnM_ura_unit (@FiniteMap.t (OneShot.t _unit))) as "H".
       iPoseProof (OwnM_Upd_set with "H") as "> [% [% OWN]]".
       { eapply FiniteMap.singleton_alloc. eapply OneShot.pending_one_wf. }
       ss. des. subst.
-      iPoseProof (white_mon with "SHOT") as "> SHOT".
-      { eapply Jacobsthal.le_mult_r.
-        eapply Ord.lt_le. apply Ord.omega_upperbound.
-      }
-      iPoseProof (Regions.alloc with "[SHOT BLACK1]") as "> [% WHITE]".
+      iPoseProof (Regions.alloc with "[SHOT PEND BLACK1]") as "> [% WHITE]".
       { instantiate (1:=(Prism.review p i, k, c, (q / 2)%Qp, k0, f)). iSplit. auto.
-        iRight. iExists _. iFrame.
+        iLeft. iFrame. iExists _. iFrame.
       }
       { iModIntro. iExists _, _. iFrame. iSplit.
         { iApply (duty_list_fold with "[DUTY] WHITE OWN"). rewrite Qp.div_2. eauto. }
@@ -1021,6 +1204,149 @@ Module ObligationRA.
       iApply (white_merge with "W1 W2").
     Qed.
 
+    Definition ptaxes (pends : nat -> option Qp) (l: list (nat * Ord.t)) (o: Ord.t): iProp :=
+      list_prop_sum (fun '(k, c) => match pends k with
+                                 | None => white k (c × o)%ord
+                                 | Some z => pending k z
+                                 end
+                    ) l.
+
+    Lemma ptaxes_perm ps l0 l1 o
+          (PERM: Permutation l0 l1)
+      :
+      ptaxes ps l0 o ⊢ ptaxes ps l1 o.
+    Proof.
+      apply list_prop_sum_perm; auto.
+    Qed.
+
+    Lemma ptaxes_nil ps o
+      :
+      ⊢ ptaxes ps [] o.
+    Proof.
+      apply list_prop_sum_nil.
+    Qed.
+
+    Lemma ptaxes_cons_fold ps k c tl o
+      :
+      ((match ps k with | None => white k (c × o)%ord | Some z => pending k z end)
+         ∗ (ptaxes ps tl o))
+        -∗
+        (ptaxes ps ((k, c)::tl) o).
+    Proof.
+      ss.
+    Qed.
+
+    Lemma ptaxes_cons_unfold ps k c tl o
+      :
+      (ptaxes ps ((k, c)::tl) o)
+        -∗
+        ((match ps k with | None => white k (c × o)%ord | Some z => pending k z end)
+           ∗ (ptaxes ps tl o)).
+    Proof.
+      ss.
+    Qed.
+
+    Lemma ptaxes_split ps l0 l1 o
+      :
+      (ptaxes ps (l0 ++ l1) o)
+        -∗
+        (ptaxes ps l0 o ∗ ptaxes ps l1 o).
+    Proof.
+      apply list_prop_sum_split.
+    Qed.
+
+    Lemma ptaxes_combine ps l0 l1 o
+      :
+      (ptaxes ps l0 o ∗ ptaxes ps l1 o)
+        -∗
+        (ptaxes ps (l0 ++ l1) o).
+    Proof.
+      apply list_prop_sum_combine.
+    Qed.
+
+    Lemma ptaxes_ord_mon ps l o0 o1
+          (LE: Ord.le o0 o1)
+      :
+      ptaxes ps l o1 ⊢ #=> ptaxes ps l o0.
+    Proof.
+      revert_until l. induction l; i.
+      { iIntros "H". iModIntro. iApply ptaxes_nil. }
+      iIntros "H". destruct a as [k o].
+      iPoseProof (ptaxes_cons_unfold with "H") as "[W TX]".
+      iPoseProof (IHl with "TX") as "IH".
+      { eauto. }
+      des_ifs.
+      { iMod "IH". iApply (ptaxes_cons_fold with "[W IH]"). rewrite Heq. iFrame. }
+      iPoseProof (white_mon with "W") as "W".
+      { instantiate (1:=(o × o0)%ord).
+        apply Jacobsthal.le_mult_r. auto.
+      }
+      iMod "W". iMod "IH".
+      iPoseProof (ptaxes_cons_fold with "[W IH]") as "A".
+      { rewrite Heq. iFrame.}
+      iModIntro. iFrame.
+    Qed.
+
+    Definition opends (pends : nat -> option Qp) (l: list (nat * Ord.t)) : iProp :=
+      list_prop_sum (fun '(k, c) => match pends k with
+                                 | None => emp%I
+                                 | Some z => pending k z
+                                 end
+                    ) l.
+
+    Lemma opends_perm ps l0 l1
+          (PERM: Permutation l0 l1)
+      :
+      opends ps l0 ⊢ opends ps l1.
+    Proof.
+      apply list_prop_sum_perm; auto.
+    Qed.
+
+    Lemma opends_nil ps
+      :
+      ⊢ opends ps [].
+    Proof.
+      apply list_prop_sum_nil.
+    Qed.
+
+    Lemma opends_cons_fold ps k c tl
+      :
+      ((match ps k with | None => emp%I | Some z => pending k z end)
+         ∗ (opends ps tl))
+        -∗
+        (opends ps ((k, c)::tl)).
+    Proof.
+      ss.
+    Qed.
+
+    Lemma opends_cons_unfold ps k c tl
+      :
+      (opends ps ((k, c)::tl))
+        -∗
+        ((match ps k with | None => emp%I | Some z => pending k z end)
+           ∗ (opends ps tl)).
+    Proof.
+      ss.
+    Qed.
+
+    Lemma opends_split ps l0 l1
+      :
+      (opends ps (l0 ++ l1))
+        -∗
+        (opends ps l0 ∗ opends ps l1).
+    Proof.
+      apply list_prop_sum_split.
+    Qed.
+
+    Lemma opends_combine ps l0 l1
+      :
+      (opends ps l0 ∗ opends ps l1)
+        -∗
+        (opends ps (l0 ++ l1)).
+    Proof.
+      apply list_prop_sum_combine.
+    Qed.
+
 
 
     Lemma duty_list_pending P i rs q
@@ -1158,25 +1484,30 @@ Module ObligationRA.
       }
       { iIntros. apply in_map_iff in IN. des. des_ifs. iApply "WHITES". auto. }
       iIntros "SAT".
-      iAssert (duty_list i rs q ∗ FairRA.black_ex p i 1%Qp ∗ (foldr (fun '(_, (_, _, _, _, f)) P => (□ (prop _ f -∗ □ prop _ f)) ∗ P) True%I rs))%I with "[DUTY BLACK SAT]" as "[DUTY [BLACK PERSS]]".
+      iAssert (duty_list i rs q ∗ FairRA.black_ex p i 1%Qp ∗ (foldr (fun '(_, (k, _, _, _, f)) P => ((□(prop _ f -∗ □ prop _ f)) ∗ (pending k (1/2) ∨ shot k)) ∗ P) emp rs))%I with "[DUTY BLACK SAT]" as "[DUTY [BLACK PERSS]]".
       { iClear "WHITES". iStopProof. clear H3. revert q. induction rs.
         { ss. i. iIntros "[[DUTY %] [BLACK _]]". ss. subst. iFrame. auto. }
         i. destruct a as [? [[[[? ?] ?] ?] ?]].
         iIntros "[DUTY [BLACK SAT]]". ss.
         iPoseProof (duty_list_unfold with "DUTY") as "[WHITE [OWN DUTY]]".
-        iDestruct "SAT" as "[[#PERS [[SHOT _]|[% [BLACK1 SAT]]]] SATS]".
-        { iExFalso. iCombine "OWN SHOT" as "OWN". iOwnWf "OWN".
-          rewrite FiniteMap.singleton_add in H3.
-          rewrite FiniteMap.singleton_wf in H3.
+        iDestruct "SAT" as "[[#PERS [(PEND & [% BLACK1] & WH) | [#SHOTk [[SHOT _]|[% [BLACK1 SAT]]]]]] SATS]".
+        - iPoseProof (IHrs with "[DUTY BLACK BLACK1 SATS]") as "[DUTY [BLACK PERSS]]".
+          { iSplitL "DUTY"; [eauto|]. iSplitL "BLACK BLACK1"; [|auto].
+            iApply (FairRA.black_ex_sum with "BLACK"). iExists _. iFrame.
+          }
+          iSplitR "BLACK PEND PERSS".
+          { iApply (duty_list_fold with "DUTY WHITE OWN"). }
+          { iFrame. auto. }
+        - iExFalso. iCombine "OWN SHOT" as "OWN". iOwnWf "OWN".
+          rewrite FiniteMap.singleton_add in H3. rewrite FiniteMap.singleton_wf in H3.
           apply OneShot.pending_not_shot in H3. ss.
-        }
-        iPoseProof (IHrs with "[DUTY BLACK BLACK1 SATS]") as "[DUTY [BLACK PERSS]]".
-        { iSplitL "DUTY"; [eauto|]. iSplitL "BLACK BLACK1"; [|auto].
-          iApply (FairRA.black_ex_sum with "BLACK"). iExists _. iFrame.
-        }
-        iSplitR "BLACK PERSS".
-        { iApply (duty_list_fold with "DUTY WHITE OWN"). }
-        { iFrame. auto. }
+        - iPoseProof (IHrs with "[DUTY BLACK BLACK1 SATS]") as "[DUTY [BLACK PERSS]]".
+          { iSplitL "DUTY"; [eauto|]. iSplitL "BLACK BLACK1"; [|auto].
+            iApply (FairRA.black_ex_sum with "BLACK"). iExists _. iFrame.
+          }
+          iSplitR "BLACK PERSS".
+          { iApply (duty_list_fold with "DUTY WHITE OWN"). }
+          { iFrame. auto. }
       }
       iPoseProof (FairRA.success_ex_update with "BLACK") as "> [[% BLACK] WHITE]".
       iFrame.
@@ -1186,7 +1517,7 @@ Module ObligationRA.
                       arrow
                       (List.map snd (List.map (fun '(r, (k, c, q0, x, f)) => (r, (Prism.review p i, k, c, q0, x, f))) rs)) ∗ FairRA.black p i a q)) with "[TAX BLACK PERSS]" as "> [REGION BLACK]".
       2:{ iModIntro. iFrame. iExists _, _. iFrame. iSplit; eauto. iExists _. iFrame. }
-      rewrite <- H4. iStopProof. clear H3 H4. revert q. induction rs.
+      iEval (rewrite <- H4) in "BLACK". iStopProof. clear H3 H4. revert q. induction rs.
       { i. iIntros "[# WHITES [TAX [BLACK PERSS]]]". iModIntro. ss. iFrame. }
       { i. iIntros "[# WHITES [TAX [BLACK PERSS]]]". ss.
         destruct a0 as [? [[[[? ?] ?] ?] ?]]. ss.
@@ -1201,7 +1532,7 @@ Module ObligationRA.
           }
         }
         iPoseProof (FairRA.black_split with "BLACK") as "[BLACK0 BLACK1]".
-        iDestruct "PERSS" as "[#PERS PERSS]".
+        iDestruct "PERSS" as "[[#PERS CASE] PERSS]".
         iPoseProof (IHrs with "[TAX BLACK1 PERSS]") as "> [REGION BLACK1]".
         { iSplit.
           { iClear "TAX BLACK1". iModIntro. iIntros.
@@ -1209,8 +1540,10 @@ Module ObligationRA.
           }
           iFrame.
         }
-        iFrame. iSplitR; [auto|]. iRight. iExists _. iFrame. iApply (white_mon with "WHITE").
-        apply Jacobsthal.le_mult_r. eapply Ord.lt_le. eapply Ord.omega_upperbound.
+        iFrame. iSplitR; [auto|]. iDestruct "CASE" as "[PEND | #SHOT]".
+        - iLeft. iFrame. iModIntro. iExists _. iFrame.
+        - iRight. iSplitR. iModIntro; auto. iRight. iExists _. iFrame. iApply (white_mon with "WHITE").
+          apply Jacobsthal.le_mult_r. eapply Ord.lt_le. eapply Ord.omega_upperbound.
       }
     Qed.
 
@@ -1235,25 +1568,30 @@ Module ObligationRA.
       iPoseProof (duty_list_whites with "DUTY") as "# WHITES".
       iIntros "SAT". iModIntro.
       iSplitL "SAT"; [auto|]. iIntros "SAT".
-      iAssert (duty_list i rs q ∗ FairRA.black_ex p i 1%Qp ∗ (foldr (fun '(_, (_, _, _, _, f)) P => (□ (prop _ f -∗ □ prop _ f)) ∗ P) True%I rs))%I with "[DUTY BLACK SAT]" as "[DUTY [BLACK PERSS]]".
+      iAssert (duty_list i rs q ∗ FairRA.black_ex p i 1%Qp ∗ (foldr (fun '(_, (k, _, _, _, f)) P => ((□(prop _ f -∗ □ prop _ f)) ∗ (pending k (1/2) ∨ shot k)) ∗ P) emp rs))%I with "[DUTY BLACK SAT]" as "[DUTY [BLACK PERSS]]".
       { iClear "WHITES". iStopProof. clear H3. revert q. induction rs.
         { ss. i. iIntros "[[DUTY %] [BLACK _]]". ss. subst. iFrame. auto. }
         i. destruct a as [? [[[[? ?] ?] ?] ?]].
         iIntros "[DUTY [BLACK SAT]]". ss.
         iPoseProof (duty_list_unfold with "DUTY") as "[WHITE [OWN DUTY]]".
-        iDestruct "SAT" as "[[#PERS [[SHOT _]|[% [BLACK1 SAT]]]] SATS]".
-        { iExFalso. iCombine "OWN SHOT" as "OWN". iOwnWf "OWN".
-          rewrite FiniteMap.singleton_add in H3.
-          rewrite FiniteMap.singleton_wf in H3.
+        iDestruct "SAT" as "[[#PERS [(PEND & [% BLACK1] & WH) | [#SHOTk [[SHOT _]|[% [BLACK1 SAT]]]]]] SATS]".
+        - iPoseProof (IHrs with "[DUTY BLACK BLACK1 SATS]") as "[DUTY [BLACK PERSS]]".
+          { iSplitL "DUTY"; [eauto|]. iSplitL "BLACK BLACK1"; [|auto].
+            iApply (FairRA.black_ex_sum with "BLACK"). iExists _. iFrame.
+          }
+          iSplitR "BLACK PEND PERSS".
+          { iApply (duty_list_fold with "DUTY WHITE OWN"). }
+          { iFrame. auto. }
+        - iExFalso. iCombine "OWN SHOT" as "OWN". iOwnWf "OWN".
+          rewrite FiniteMap.singleton_add in H3. rewrite FiniteMap.singleton_wf in H3.
           apply OneShot.pending_not_shot in H3. ss.
-        }
-        iPoseProof (IHrs with "[DUTY BLACK BLACK1 SATS]") as "[DUTY [BLACK PERSS]]".
-        { iSplitL "DUTY"; [eauto|]. iSplitL "BLACK BLACK1"; [|auto].
-          iApply (FairRA.black_ex_sum with "BLACK"). iExists _. iFrame.
-        }
-        iSplitR "BLACK PERSS".
-        { iApply (duty_list_fold with "DUTY WHITE OWN"). }
-        { iFrame. auto. }
+        - iPoseProof (IHrs with "[DUTY BLACK BLACK1 SATS]") as "[DUTY [BLACK PERSS]]".
+          { iSplitL "DUTY"; [eauto|]. iSplitL "BLACK BLACK1"; [|auto].
+            iApply (FairRA.black_ex_sum with "BLACK"). iExists _. iFrame.
+          }
+          iSplitR "BLACK PERSS".
+          { iApply (duty_list_fold with "DUTY WHITE OWN"). }
+          { iFrame. auto. }
       }
       iModIntro. iSplitL "BLACK"; [auto|].
       iAssert (⌜(fold_right (fun '(r, (k, c, q0, x, f)) q1 => (q0 + q1)%Qp) q rs = 1%Qp)⌝)%I as "%".
@@ -1263,7 +1601,7 @@ Module ObligationRA.
                       arrow
                       (List.map snd (List.map (fun '(r, (k, c, q0, x, f)) => (r, (Prism.review p i, k, c, q0, x, f))) rs)) ∗ FairRA.black p i a q)) with "[TAX BLACK PERSS]" as "> [REGION BLACK]".
       2:{ iModIntro. iFrame. iExists _. eauto. }
-      rewrite <- H4. iStopProof. clear H3 H4. revert q. induction rs.
+      iEval (rewrite <- H4) in "BLACK". iStopProof. clear H3 H4. revert q. induction rs.
       { i. iIntros "[# WHITES [TAX [BLACK PERSS]]]". iModIntro. ss. iFrame. }
       { i. iIntros "[# WHITES [TAX [BLACK PERSS]]]". ss.
         destruct a0 as [? [[[[? ?] ?] ?] ?]]. ss.
@@ -1278,7 +1616,7 @@ Module ObligationRA.
           }
         }
         iPoseProof (FairRA.black_split with "BLACK") as "[BLACK0 BLACK1]".
-        iDestruct "PERSS" as "[#PERS PERSS]".
+        iDestruct "PERSS" as "[(#PERS & CASE) PERSS]".
         iPoseProof (IHrs with "[TAX BLACK1 PERSS]") as "> [REGION BLACK1]".
         { iSplit.
           { iClear "TAX BLACK1". iModIntro. iIntros.
@@ -1286,8 +1624,10 @@ Module ObligationRA.
           }
           iFrame.
         }
-        iFrame. iSplitR. auto. iRight. iExists _. iFrame. iApply (white_mon with "WHITE").
-        apply Jacobsthal.le_mult_r. eapply Ord.lt_le. eapply Ord.omega_upperbound.
+        iFrame. iSplitR. auto. iDestruct "CASE" as "[PEND | #SHOTk]".
+        - iLeft. iFrame. iModIntro. iExists _. iFrame.
+        - iRight. iSplitR. iModIntro; auto. iRight. iExists _. iFrame. iApply (white_mon with "WHITE").
+          apply Jacobsthal.le_mult_r. eapply Ord.lt_le. eapply Ord.omega_upperbound.
       }
     Qed.
 
@@ -1380,8 +1720,6 @@ Module ObligationRA.
         iAssert (#=(arrows_sat)=>
                    (((duty_list i rs q)
                        ∗
-                       (* (foldr (fun '(_, (_, _, _, _, f)) P => (□ (prop _ f -∗ □ prop _ f)) ∗ P) True%I rs) *)
-                       (* ∗ *)
                        (list_prop_sum (fun '(i, rs, q) =>
                                          (duty_list i rs q)
                                            ∗
@@ -1477,6 +1815,289 @@ Module ObligationRA.
         iPoseProof (Regions.sat_list_combine with "SATS") as "SATS". iFrame.
       }
       { iFrame. iExists _, _. iFrame. eauto. }
+    Qed.
+
+    Lemma duty_list_updating_pending i rs q (pends : nat -> option Qp)
+      :
+      (duty_list i rs q)
+        -∗
+        (FairRA.black_ex p i q)
+        -∗
+        (list_prop_sum (fun '(r, (k, c, q, x, f)) => match pends k with
+                                                  | None => (white k (c × Ord.omega)%ord)
+                                                  | Some z => (pending k z)
+                                                  end) rs)
+        -∗
+        #=(arrows_sat)=>
+            (updating
+               (@Regions.sat_list _ (fun l => (S * nat * Ord.t * Qp * nat * (Vars l))%type) _ _ arrow (List.map snd (List.map (fun '(r, (k, c, q, x, f)) => (r, (Prism.review p i, k, c, q, x, f))) rs)))
+               (FairRA.black_ex p i 1)
+               (FairRA.black_ex p i 1)
+               ((duty_list i rs q)
+                  ∗ (FairRA.black_ex p i q)
+                  ∗ (list_prop_sum (fun '(r, (k, c, q, x, f)) => match pends k with
+                                                              | None => emp
+                                                              | Some z => (pending k z)
+                                                              end) rs)
+            )).
+    Proof.
+      iIntros "DUTY BLACK TAX".
+      iPoseProof (duty_list_nodup with "DUTY") as "> [DUTY %]".
+      { reflexivity. }
+      iPoseProof (duty_list_whites with "DUTY") as "# WHITES".
+      iIntros "SAT". iModIntro.
+      iSplitL "SAT"; [auto|]. iIntros "SAT".
+      iAssert (duty_list i rs q ∗ FairRA.black_ex p i 1%Qp ∗ (foldr (fun '(_, (k, c, _, _, f)) P => ((□(prop _ f -∗ □ prop _ f)) ∗ ((pending k (1/2) ∗ white k (c × Ord.omega)%ord) ∨ shot k)) ∗ P) emp rs))%I with "[DUTY BLACK SAT]" as "[DUTY [BLACK PERSS]]".
+      { iClear "WHITES". iStopProof. clear H3. revert q. induction rs.
+        { ss. i. iIntros "[[DUTY %] [BLACK _]]". ss. subst. iFrame. auto. }
+        i. destruct a as [? [[[[? ?] ?] ?] ?]].
+        iIntros "[DUTY [BLACK SAT]]". ss.
+        iPoseProof (duty_list_unfold with "DUTY") as "[WHITE [OWN DUTY]]".
+        iDestruct "SAT" as "[[#PERS [(PEND & [% BLACK1] & WH) | [#SHOTk [[SHOT _]|[% [BLACK1 SAT]]]]]] SATS]".
+        - iPoseProof (IHrs with "[DUTY BLACK BLACK1 SATS]") as "[DUTY [BLACK PERSS]]".
+          { iSplitL "DUTY"; [eauto|]. iSplitL "BLACK BLACK1"; [|auto].
+            iApply (FairRA.black_ex_sum with "BLACK"). iExists _. iFrame.
+          }
+          iSplitR "BLACK PEND WH PERSS".
+          { iApply (duty_list_fold with "DUTY WHITE OWN"). }
+          { iFrame. iSplitR. auto. iLeft. iFrame. }
+        - iExFalso. iCombine "OWN SHOT" as "OWN". iOwnWf "OWN".
+          rewrite FiniteMap.singleton_add in H3. rewrite FiniteMap.singleton_wf in H3.
+          apply OneShot.pending_not_shot in H3. ss.
+        - iPoseProof (IHrs with "[DUTY BLACK BLACK1 SATS]") as "[DUTY [BLACK PERSS]]".
+          { iSplitL "DUTY"; [eauto|]. iSplitL "BLACK BLACK1"; [|auto].
+            iApply (FairRA.black_ex_sum with "BLACK"). iExists _. iFrame.
+          }
+          iSplitR "BLACK PERSS".
+          { iApply (duty_list_fold with "DUTY WHITE OWN"). }
+          { iFrame. auto. }
+      }
+      iModIntro. iSplitL "BLACK"; [auto|].
+      iAssert (⌜(fold_right (fun '(r, (k, c, q0, x, f)) q1 => (q0 + q1)%Qp) q rs = 1%Qp)⌝)%I as "%".
+      { iPoseProof "DUTY" as "[DUTY %]". auto. }
+      iIntros "[% BLACK]".
+      iAssert (#=> ((Region.sat_list
+                       arrow
+                       (List.map snd (List.map (fun '(r, (k, c, q0, x, f)) => (r, (Prism.review p i, k, c, q0, x, f))) rs)))
+                      ∗ (FairRA.black p i a q)
+                      ∗ (list_prop_sum (λ '(_, (k, _, _, _, _)), match pends k with
+                                                                 | Some z => pending k z
+                                                                 | None => emp%I
+                                                                 end) rs)
+              )) with "[TAX BLACK PERSS]" as "> (REGION & BLACK & PENDS)".
+      2:{ iModIntro. iFrame. iExists _. eauto. }
+      iEval (rewrite <- H4) in "BLACK". iStopProof. clear H3 H4. revert q. induction rs.
+      { i. iIntros "[# WHITES [TAX [BLACK PERSS]]]". iModIntro. ss. iFrame. }
+      { i. iIntros "[# WHITES [TAX [BLACK PERSS]]]". ss.
+        destruct a0 as [? [[[[? ?] ?] ?] ?]]. ss.
+        iPoseProof "TAX" as "[WHITE TAX]".
+        replace (q0 + foldr (fun '(_, (_, _, q1, _, _)) q2 => (q1 + q2)%Qp) q rs)%Qp with (q + foldr (fun '(_, (_, _, q1, _, _)) q2 => (q1 + q2)%Qp) q0 rs)%Qp; cycle 1.
+        { clear IHrs. revert q q0. induction rs; ss; i.
+          { apply Qp.add_comm. }
+          { destruct a0 as [? [[[[? ?] ?] ?] ?]].
+            rewrite (IHrs q1 q0). rewrite (IHrs q1 q).
+            rewrite Qp.add_assoc. rewrite Qp.add_assoc.
+            f_equal. apply Qp.add_comm.
+          }
+        }
+        iPoseProof (FairRA.black_split with "BLACK") as "[BLACK0 BLACK1]".
+        iDestruct "PERSS" as "[(#PERS & CASE) PERSS]".
+        iPoseProof (IHrs with "[TAX BLACK1 PERSS]") as "> (REGION & BLACK1 & PENDS)".
+        { iSplit.
+          { iClear "TAX BLACK1". iModIntro. iIntros.
+            iApply "WHITES". eauto.
+          }
+          iFrame.
+        }
+        iFrame. destruct (pends n0) eqn:PENDS.
+        - iDestruct "CASE" as "[(PEND & WHI) | #SHOTk]".
+          + iFrame. iSplitR. iModIntro; auto. iLeft. iFrame. iModIntro. iExists _. iFrame.
+          + iPoseProof (pending_not_shot with "WHITE SHOTk") as "%FAL". inv FAL.
+        - iDestruct "CASE" as "[(PEND & WHI) | #SHOTk]".
+          + iSplitL; [|auto]. iSplitR; [auto|]. iLeft. iFrame. iModIntro. iExists _. iFrame.
+          + iSplitL; [|auto]. iSplitR; [auto|].
+            iRight. iSplitR. iModIntro; auto. iRight. iExists _. iFrame. iApply (white_mon with "WHITE").
+            apply Jacobsthal.le_mult_r. eapply Ord.lt_le. eapply Ord.omega_upperbound.
+      }
+    Qed.
+
+    Lemma duties_updating_pending os (pends : nat -> option Qp)
+      :
+      (list_prop_sum (fun '(i, l) => duty i l ∗ ptaxes pends (map fst l) Ord.omega) os)
+        -∗
+        #=(arrows_sat)=>
+            (updating
+               arrows_sat
+               (FairRA.blacks_of p (List.map fst os))
+               (FairRA.blacks_of p (List.map fst os))
+               (list_prop_sum (fun '(i, l) => duty i l ∗ opends pends (map fst l)) os)).
+    Proof.
+      iIntros "DUTY".
+      iAssert (∃ (xs: list (Id * list (nat * (nat * Ord.t * Qp * nat * Var)) * Qp)),
+                  (⌜os = List.map (fun '(i, rs, q) => (i, List.map (fun '(r, (k, c, q, x, f)) => (k, c, f)) rs)) xs⌝)
+                    ∗
+                    (#=(arrows_sat)=> list_prop_sum (fun '(i, rs, q) =>
+                                                      (duty_list i rs q)
+                                                        ∗
+                                                        (list_prop_sum (fun '(r, (k, c, q, x, f)) =>
+                                                                          match pends k with
+                                                                          | None => (white k (c × Ord.omega)%ord)
+                                                                          | Some z => (pending k z)
+                                                                          end) rs)
+                                                        ∗
+                                                        (FairRA.black_ex p i q)
+                                                        ∗
+                                                        (foldr (fun '(_, (_, _, _, _, f)) P => (□ (prop _ f -∗ □ prop _ f)) ∗ P) True%I rs)) xs))%I with "[DUTY]" as "[% [% >ALL]]".
+      { iStopProof. induction os; ss; i.
+        { iIntros. iExists []. ss. }
+        { destruct a as [i l].
+          iIntros "[[[% [% [BLACK [DUTY %]]]] TAX] OS]".
+          iPoseProof (IHos with "OS") as "[% [% OS]]". subst.
+          iExists ((_, _, _)::_). ss. iSplit.
+          { iPureIntro. eauto. }
+          iMod "OS".
+          iPoseProof (duty_list_pers_props with "DUTY") as ">[DUTY #PERSS]".
+          iFrame. iSplitL. 2: auto. clear IHos. iClear "PERSS". iStopProof. induction rs; ss.
+          { auto. }
+          destruct a as [? [[[[? ?] ?] ?] ?]].
+          iIntros "TAX". iPoseProof (ptaxes_cons_unfold with "TAX") as "[HD TL]".
+          iFrame. iPoseProof (IHrs with "TL") as "TL". iFrame.
+        }
+      }
+      subst.
+      set (l := List.concat (List.map (fun '(i, rs, q) => List.map (fun '(r, (k, c, q, x, f)) => (r, (Prism.review p i, k, c, q, x, f))) rs) xs)).
+
+      iAssert (#=(arrows_sat)=>
+                 ((list_prop_sum (fun '(i, rs, q) =>
+                                    (duty_list i rs q)
+                                      ∗
+                                      (list_prop_sum (fun '(r, (k, c, q, x, f)) =>
+                                                        match pends k with
+                                                        | None => (white k (c × Ord.omega)%ord)
+                                                        | Some z => (pending k z)
+                                                        end) rs)
+                                      ∗
+                                      (FairRA.black_ex p i q)
+                                      ∗
+                                      (foldr (fun '(_, (_, _, _, _, f)) P => (□ (prop _ f -∗ □ prop _ f)) ∗ P) True%I rs)) xs)
+                    ∗
+                    (⌜List.NoDup (List.map fst l)⌝))%I) with "[ALL]" as "> [ALL %]".
+      { subst l. iStopProof. induction xs; ss.
+        { iIntros. iModIntro. iSplit; ss. iPureIntro. econs; ss. }
+        destruct a as [[i rs] q]. iIntros "[[DUTY [HD BLACK]] TL]".
+        iPoseProof (IHxs with "TL") as "> [TL %]".
+        iPoseProof (duty_list_nodup with "DUTY") as "> [DUTY %]".
+        { reflexivity. }
+        iAssert (#=(arrows_sat)=>
+                   (((duty_list i rs q)
+                       ∗
+                       (list_prop_sum (fun '(i, rs, q) =>
+                                         (duty_list i rs q)
+                                           ∗
+                                           (list_prop_sum (fun '(r, (k, c, q, x, f)) =>
+                                                             match pends k with
+                                                             | None => (white k (c × Ord.omega)%ord)
+                                                             | Some z => (pending k z)
+                                                             end) rs)
+                                           ∗
+                                           (FairRA.black_ex p i q)
+                                           ∗
+                                           (foldr (fun '(_, (_, _, _, _, f)) P => (□ (prop _ f -∗ □ prop _ f)) ∗ P) True%I rs)) xs))
+                      ∗
+                      (⌜forall i0 rs0 q0 (IN: List.In (i0, rs0, q0) xs),
+                            (forall r (IN0: List.In r (List.map fst rs)) (IN1: List.In r (List.map fst rs0)), False)⌝)))%I with "[DUTY TL]" as "> [[DUTY TL] %]".
+        { clear IHxs H3 H4. iStopProof. induction xs; ss.
+          { iIntros "[DUTY TL]". iModIntro. iSplit; auto. }
+          destruct a as [[i0 rs0] q0].
+          iIntros "[DUTY [HD TL]]".
+          iPoseProof (IHxs with "[DUTY TL]") as "> [[DUTY TL] %]".
+          { iFrame. }
+          iCombine "HD DUTY" as "H".
+          iPoseProof (duty_list_disjoint with "H") as "> [[HD DUTY] %]".
+          { iIntros "[[[H0 X0] X1] H1]". iFrame. }
+          iModIntro. iFrame. iPureIntro. i. des; clarify; eauto.
+        }
+        { iModIntro. iFrame. iPureIntro.
+          rewrite List.map_app. apply list_app_disjoint_nodup; auto.
+          { rewrite List.map_map. erewrite List.map_ext; eauto. i. des_ifs. }
+          { i. rewrite List.concat_map in IN1.
+            apply in_concat in IN1. des.
+            rewrite List.map_map in IN1. rewrite List.in_map_iff in IN1. des. subst.
+            rewrite List.in_map_iff in IN2. des. subst.
+            destruct x0 as [[? ?] ?].
+            rewrite List.in_map_iff in IN1. des. subst.
+            destruct x0 as [? [[[[? ?] ?] ?] ?]]. ss.
+            rewrite List.map_map in IN0.
+            rewrite List.in_map_iff in IN0. des. subst.
+            destruct x as [? [[[[? ?] ?] ?] ?]]. ss.
+            eapply H5.
+            { eauto. }
+            { eapply in_map_iff. esplits; eauto. }
+            { ss. eapply in_map_iff. esplits; eauto. ss. }
+          }
+        }
+      }
+      iAssert (#=(arrows_sat)=>
+                 (((list_prop_sum (fun '(i, rs, q) =>
+                                     (updating
+                                        (@Regions.sat_list _ (fun l => (S * nat * Ord.t * Qp * nat * (Vars l))%type) _ _ arrow (List.map snd (List.map (fun '(r, (k, c, q, x, f)) => (r, (Prism.review p i, k, c, q, x, f))) rs)))
+                                        (FairRA.black_ex p i 1)
+                                        (FairRA.black_ex p i 1)
+                                        (duty_list i rs q ∗ FairRA.black_ex p i q
+                                                   ∗ (list_prop_sum (fun '(r, (k, c, q, x, f)) => match pends k with
+                                                                                               | None => emp
+                                                                                               | Some z => (pending k z)
+                                                                                               end) rs)
+                                     ))%I)) xs)
+                    ∗ (∀ i rs q0 r k c q1 x f
+                         (IN0: List.In (i, rs, q0) xs)
+                         (IN1: List.In (r, (k, c, q1, x, f)) rs),
+                          @Regions.white _ (fun l => (S * nat * Ord.t * Qp * nat * (Vars l))%type) _ _ _ r (Prism.review p i, k, c, q1, x, f)))) with "[ALL]" as "> [ALL WHITES]".
+      { subst l. iStopProof. clear H3. induction xs.
+        { iIntros. iModIntro. ss. iSplit; auto. iIntros. ss. }
+        destruct a as [[i rs] q]. iIntros "[[DUTY [TAX [BLACK PERSS]]] DUTIES]".
+        iPoseProof (IHxs with "DUTIES") as "> [DUTIES WHITES]".
+        iPoseProof (duty_list_whites with "DUTY") as "# WHITE".
+        iPoseProof (duty_list_updating_pending with "DUTY BLACK TAX") as "> UPD".
+        iModIntro. iSplitL "DUTIES UPD".
+        { ss. iFrame. }
+        { iIntros. ss. des; clarify.
+          { iApply "WHITE"; auto. }
+          { iApply "WHITES"; auto. }
+        }
+      }
+      iModIntro.
+      iApply (Regions.sat_updating with "[WHITES] [ALL]").
+      { instantiate (1:=l). subst l. auto. }
+      { iIntros. subst l. apply List.in_concat in IN. des.
+        apply in_map_iff in IN. des. destruct x0 as [[i rs] q]. subst.
+        apply in_map_iff in IN0. des.
+        destruct x as [? [[[[? ?] ?] ?] ?]]. clarify.
+        iApply "WHITES"; eauto.
+      }
+      subst l. clear H3. iStopProof. induction xs.
+      { ss. iIntros "_ SAT". iModIntro. ss. }
+      destruct a as [[i rs] q]. ss.
+      iIntros "[UPD UPDS]".
+      iPoseProof (IHxs with "UPDS") as "UPDS".
+      iIntros "SAT". repeat rewrite List.map_app.
+      iPoseProof (Regions.sat_list_split with "SAT") as "[SAT SATS]".
+      iPoseProof ("UPD" with "SAT") as "> [BLACK K]".
+      iPoseProof ("UPDS" with "SATS") as "> [BLACKS KS]".
+      iModIntro. iSplitL "BLACK BLACKS".
+      { iApply list_prop_sum_cons_fold. iFrame. }
+      iIntros "BLACKS".
+      iPoseProof (list_prop_sum_cons_unfold with "BLACKS") as "[BLACK BLACKS]".
+      iPoseProof ("K" with "BLACK") as "> [SAT [BLACK [DUTY PENDS]]]".
+      iPoseProof ("KS" with "BLACKS") as "> [SATS DUTIES]".
+      iModIntro. iSplitL "SAT SATS".
+      { iCombine "SAT SATS" as "SATS".
+        iPoseProof (Regions.sat_list_combine with "SATS") as "SATS". iFrame.
+      }
+      { iFrame. iSplitR "PENDS". iExists _, _. iFrame. eauto. unfold opends.
+        iEval (rewrite map_map). iApply list_prop_sum_map. 2: iFrame.
+        ss. i. des_ifs.
+      }
     Qed.
 
     End PRISM.
